\documentclass{article}
\usepackage{epsfig}
\pagestyle{empty}
\begin{document}
$ Ax = b $
\pagebreak

$ A $
\pagebreak

$ Ax=b $
\pagebreak

$ A = QR $
\pagebreak

$ A = RQ $
\pagebreak

$ A = QL $
\pagebreak

$ A = LQ $
\pagebreak

$ Ax = \lambda x $
\pagebreak

$ Ax = \lambda Bx $
\pagebreak

$ ABx = \lambda x $
\pagebreak

$ BAx = \lambda x $
\pagebreak

$ A = U \Sigma V^T $
\pagebreak

$ O(n) $
\pagebreak

$ O(n^2) $
\pagebreak

$ O(n^3) $
\pagebreak

$ O(1) $
\pagebreak

$ x^H y $
\pagebreak

$ x^T y $
\pagebreak

$ y = \alpha x + y $
\pagebreak

$ \alpha $
\pagebreak

$ y = x $
\pagebreak

$ x = \alpha x $
\pagebreak

$ x <-> y $
\pagebreak

$ y = \alpha A x + \beta y $
\pagebreak

$ y = \alpha A^T x + \beta y $
\pagebreak

$ y = \alpha A^H x + \beta y $
\pagebreak

$ \beta $
\pagebreak

$ A = \alpha x y^H + A $
\pagebreak

$ A = \alpha x x^H + A $
\pagebreak

$ A = \alpha x y^H + conj(\alpha) y x^H + A $
\pagebreak

$ x = A x $
\pagebreak

$ x = A^T x $
\pagebreak

$ x = A^H x $
\pagebreak

$ A x = b $
\pagebreak

$ A^T x = b $
\pagebreak

$ A^H x = b $
\pagebreak

$ C = \alpha op(A) op(B) + \beta C $
\pagebreak

$ C = \alpha A B + \beta C $
\pagebreak

$ C = \alpha B A + \beta C $
\pagebreak

$ C = \alpha A A^T + \beta C $
\pagebreak

$ C = \alpha A^T A + \beta C $
\pagebreak

$ C $
\pagebreak

$ C = \alpha A B^T + \alpha B A^T \beta C $
\pagebreak

$ C = \alpha A^T B + \alpha B^T A \beta C $
\pagebreak

$ B = \alpha op(A) B $
\pagebreak

$ B = \alpha B op(A) $
\pagebreak

$ op(A) X = \alpha B $
\pagebreak

$ X op(A) = \alpha B $
\pagebreak

\end{document}
